Work in progress abssem

vipersemabstract/AbstractSemantics.thy
@@ -4,7 +4,7 @@ begin
 
 section Start
 
-type_synonym 'a assertion = "'a \<Rightarrow> bool"
+type_synonym 'a assertion = "'a set"
 
 
 type_synonym 'a bexp = "'a \<rightharpoonup> bool"
@@ -55,6 +55,8 @@ locale semantics =
 (* Axioms
 - TODO: Add smth about has_value
 *)
+
+(* Needed? *)
   assumes frame_preserving_writing_orig: "Some x = a \<oplus> b \<Longrightarrow> stable b \<Longrightarrow> has_write_perm_only a hl \<Longrightarrow> Some (set_value x hl v) = set_value a hl v \<oplus> b"
       and has_write_perm_only_same: "has_write_perm_only a hl \<Longrightarrow> has_write_perm_only b hl \<Longrightarrow> stabilize a = stabilize b"
   (* TODO: WRONG! Needs something about the value! *)
@@ -73,23 +75,38 @@ begin
 definition has_write_perm :: "'a \<Rightarrow> 'r \<Rightarrow> bool" where
   "has_write_perm x hl \<longleftrightarrow> (\<exists>r. x \<succeq> r \<and> has_write_perm_only r hl)"
 
-definition inh ("\<langle>_\<rangle>" [51] 81) where
-  "\<langle>A\<rangle> = { \<omega> |\<omega>. A \<omega> }"
-
 definition filter_dom where
   "filter_dom vars S = Set.filter (\<lambda>\<omega>. dom (get_store \<omega>) = vars) S"
 
+(*
 definition self_framing :: "(('v, 'a) abs_state \<Rightarrow> bool) \<Rightarrow> bool" where
   "self_framing A \<longleftrightarrow> (\<forall>\<omega>. A \<omega> \<longleftrightarrow> A (stabilize \<omega>))"
+*)
 
+(*
+lemma "Stable A \<longleftrightarrow> (\<forall>\<omega>. \<omega> \<in> A \<longleftrightarrow> stabilize \<omega> \<in> A)" (is "?P \<longleftrightarrow> ?Q")
+proof -
+  have "?P \<longleftrightarrow> A \<subseteq> {\<omega>. stabilize \<omega> \<in> A}" unfolding Stable_def Stabilize_def by blast
+  also have "... \<longleftrightarrow> (\<forall>\<omega>. \<omega> \<in> A \<longrightarrow> stabilize \<omega> \<in> A)"
+    by blast
+\<omega> \<notin> A \<longrightarrow> stabilize \<omega> \<notin> A
+
+
+
+definition Stable :: "'a set \<Rightarrow> bool" where
+  "Stable A \<longleftrightarrow> (A \<subseteq> Stabilize A)"
+*)
+
+thm Stable_def
+thm Stabilize_def (* Stabilize ?A = {\<omega>. stabilize \<omega> \<in> ?A} *)
 
 text \<open>The truth of A in a only depends on parts of a (for a ## \<omega>) that:
 1) are stable, or
 2) are given by |\<omega>|\<close>
 definition rel_stable_assertion where
 (*  "rel_stable_assertion \<omega> A \<longleftrightarrow> (\<forall>\<omega>'. \<omega> ## \<omega>' \<longrightarrow> (A \<omega>' \<longleftrightarrow> A (stabilize_rel \<omega> \<omega>')))" *)
-  "rel_stable_assertion \<omega> A \<longleftrightarrow> (\<forall>x a. \<omega> ## a \<and> pure_larger x (stabilize a) \<and> x \<succeq> |\<omega>| \<longrightarrow> (A a \<longleftrightarrow> A x))"
-
+  "rel_stable_assertion \<omega> A \<longleftrightarrow> (\<forall>x a. \<omega> ## a \<and> pure_larger x (stabilize a) \<and> x \<succeq> |\<omega>| \<longrightarrow> (a \<in> A \<longleftrightarrow> x \<in> A))"
+(* TODO: Think about it *)
 
 section \<open>Operational semantics\<close>
 
@@ -102,14 +119,12 @@ where
 
 | RedSkip: "red_stmt \<Delta> Skip \<omega> ({\<omega>})"
 
-| RedAssertTrue: "\<lbrakk> A \<omega> \<rbrakk> \<Longrightarrow> red_stmt \<Delta> (Assert A) \<omega> ({\<omega>})"
-| RedAssumeTrue: "\<lbrakk> rel_stable_assertion \<omega> A; A \<omega> \<rbrakk> \<Longrightarrow> red_stmt \<Delta> (Assume A) \<omega> ({\<omega>})"
-| RedAssumeFalse: "\<lbrakk> rel_stable_assertion \<omega> A; \<not> A \<omega> \<rbrakk> \<Longrightarrow> red_stmt \<Delta> (Assume A) \<omega> ({})"
+| RedAssertTrue: "\<lbrakk> \<omega> \<in> A \<rbrakk> \<Longrightarrow> red_stmt \<Delta> (Assert A) \<omega> ({\<omega>})"
+| RedAssumeTrue: "\<lbrakk> rel_stable_assertion \<omega> A; \<omega> \<in> A \<rbrakk> \<Longrightarrow> red_stmt \<Delta> (Assume A) \<omega> ({\<omega>})"
+| RedAssumeFalse: "\<lbrakk> rel_stable_assertion \<omega> A; \<omega> \<notin> A \<rbrakk> \<Longrightarrow> red_stmt \<Delta> (Assume A) \<omega> ({})"
 
-
-
-| RedInhale: "\<lbrakk> rel_stable_assertion \<omega> A \<rbrakk> \<Longrightarrow> red_stmt \<Delta> (Inhale A) \<omega> (Set.filter stable ({\<omega>} \<otimes> \<langle>A\<rangle>))"
-| RedExhale: "\<lbrakk> a \<in> \<langle>A\<rangle> ; Some \<omega> = \<omega>' \<oplus> a ; stable \<omega>' \<rbrakk> \<Longrightarrow> red_stmt \<Delta> (Exhale A) \<omega> {\<omega>'}"
+| RedInhale: "\<lbrakk> rel_stable_assertion \<omega> A \<rbrakk> \<Longrightarrow> red_stmt \<Delta> (Inhale A) \<omega> (Set.filter stable ({\<omega>} \<otimes> A))"
+| RedExhale: "\<lbrakk> a \<in> A ; Some \<omega> = \<omega>' \<oplus> a ; stable \<omega>' \<rbrakk> \<Longrightarrow> red_stmt \<Delta> (Exhale A) \<omega> {\<omega>'}"
 
 | RedIfTrue: "\<lbrakk> b \<omega> = Some True ; red_stmt \<Delta> C1 \<omega> S \<rbrakk> \<Longrightarrow> red_stmt \<Delta> (If b C1 C2) \<omega> S"
 | RedIfFalse: "\<lbrakk> b \<omega> = Some False ; red_stmt \<Delta> C2 \<omega> S \<rbrakk> \<Longrightarrow> red_stmt \<Delta> (If b C1 C2) \<omega> S"
@@ -154,6 +169,10 @@ where
 Needs type context to havoc
 *)
 
+definition self_framing where
+  "self_framing A \<longleftrightarrow> (\<forall>\<omega>. \<omega> \<in> A \<longleftrightarrow> stabilize \<omega> \<in> A)"
+
+
 definition typed_store :: "('v, 'r) abs_type_context \<Rightarrow> (var \<rightharpoonup> 'v) \<Rightarrow> bool" where
   "typed_store \<Delta> \<sigma> \<longleftrightarrow> (dom (variables \<Delta>) = dom \<sigma> \<and> (\<forall>x v ty. \<sigma> x = Some v \<and> variables \<Delta> x = Some ty \<longrightarrow> v \<in> ty))"
 
@@ -162,19 +181,19 @@ section \<open>Assertions\<close>
 subsection \<open>General concepts\<close>
 
 definition framed_by :: "('v, 'a) abs_state assertion \<Rightarrow> ('v, 'a) abs_state assertion \<Rightarrow> bool" where
-  "framed_by A B \<longleftrightarrow> (\<forall>\<omega> \<in> \<langle>A\<rangle>. stable \<omega> \<longrightarrow> rel_stable_assertion \<omega> B)"
+  "framed_by A B \<longleftrightarrow> (\<forall>\<omega> \<in> A. stable \<omega> \<longrightarrow> rel_stable_assertion \<omega> B)"
 
 definition wf_exp where
   "wf_exp e \<longleftrightarrow> (\<forall>a b v. a \<succeq> b \<and> e b = Some v \<longrightarrow> e a = Some v) \<and> (\<forall>a. e a = e |a| )"
 
 definition framed_by_exp where
-  "framed_by_exp A e \<longleftrightarrow> (\<forall>\<omega> \<in> \<langle>A\<rangle>. e \<omega> \<noteq> None)"
+  "framed_by_exp A e \<longleftrightarrow> (\<forall>\<omega> \<in> A. e \<omega> \<noteq> None)"
 
 definition entails where
-  "entails A B \<longleftrightarrow> \<langle>A\<rangle> \<subseteq> \<langle>B\<rangle>"
+  "entails A B \<longleftrightarrow> A \<subseteq> B"
 
 definition equiv where
-  "equiv A B \<longleftrightarrow> \<langle>A\<rangle> = \<langle>B\<rangle>"
+  "equiv A B \<longleftrightarrow> A = B"
 
 
 
@@ -184,7 +203,7 @@ definition equal_on_set :: "var set \<Rightarrow> (var \<rightharpoonup> 'v) \<R
   "equal_on_set S \<sigma>1 \<sigma>2 \<longleftrightarrow> (\<forall>x \<in> S. \<sigma>1 x = \<sigma>2 x)"
 
 definition overapprox_fv :: "('v, 'r) abs_type_context \<Rightarrow> ('v, 'a) abs_state assertion \<Rightarrow> var set \<Rightarrow> bool" where
-  "overapprox_fv \<Delta> A S \<longleftrightarrow> (\<forall>\<sigma>1 \<sigma>2 \<tau> \<gamma>. typed_store \<Delta> \<sigma>1 \<and> typed_store \<Delta> \<sigma>2 \<and> equal_on_set S \<sigma>1 \<sigma>2 \<longrightarrow> (A ((Ag \<sigma>1, \<tau>), \<gamma>) \<longleftrightarrow> A ((Ag \<sigma>2, \<tau>), \<gamma>)))"
+  "overapprox_fv \<Delta> A S \<longleftrightarrow> (\<forall>\<sigma>1 \<sigma>2 \<tau> \<gamma>. typed_store \<Delta> \<sigma>1 \<and> typed_store \<Delta> \<sigma>2 \<and> equal_on_set S \<sigma>1 \<sigma>2 \<longrightarrow> (((Ag \<sigma>1, \<tau>), \<gamma>) \<in> A \<longleftrightarrow> ((Ag \<sigma>2, \<tau>), \<gamma>) \<in> A))"
 
 
 definition free_vars where
@@ -196,11 +215,10 @@ definition at_least_two_elems:
   "at_least_two_elems S \<longleftrightarrow> (\<exists>a b. a \<in> S \<and> b \<in> S \<and> a \<noteq> b)"
 
 subsection \<open>wf_assertion\<close>
-
+(*
 (* TODO: Is it needed? *)
 definition wf_assertion :: "('v, 'a) abs_state assertion \<Rightarrow> bool" where
   "wf_assertion A \<longleftrightarrow> (\<forall>x' x. pure_larger x' x \<and> A x \<longrightarrow> A x')"
-
 
 fun wf_abs_stmt where
   "wf_abs_stmt \<Delta> Skip \<longleftrightarrow> True"
@@ -215,7 +233,7 @@ fun wf_abs_stmt where
 | "wf_abs_stmt \<Delta> (Havoc x) \<longleftrightarrow> x \<in> dom (variables \<Delta>)"
 | "wf_abs_stmt \<Delta> (Label _) \<longleftrightarrow> True" (* TODO: Prevent duplicate labels? *)
 | "wf_abs_stmt \<Delta> (Scope _ C) \<longleftrightarrow> wf_abs_stmt \<Delta> C" (* TODO: Prevent duplicate labels? *)
-
+*)
 
 fun modif where
   "modif (LocalAssign x _) = {x}"
@@ -232,12 +250,12 @@ fun havoc_list where
 
 subsection \<open>Assertion connectives\<close>
 
-definition pure_assertify where
-  "pure_assertify b \<omega> \<longleftrightarrow> b \<omega> = Some True"
+definition pure_Stabilize where
+  "pure_Stabilize b \<omega> \<longleftrightarrow> b \<omega> = Some True"
 
 definition negate where
   "negate b \<omega> = (if b \<omega> = None then None else Some (\<not> (the (b \<omega>))))"
-
+(*
 definition astar :: "('v, 'a) abs_state assertion \<Rightarrow> ('v, 'a) abs_state assertion \<Rightarrow> ('v, 'a) abs_state assertion"
  (infixl "&&" 60)
   where
@@ -251,21 +269,20 @@ definition aconj :: "('v, 'a) abs_state assertion \<Rightarrow> ('v, 'a) abs_sta
 
 definition adisj :: "('v, 'a) abs_state assertion \<Rightarrow> ('v, 'a) abs_state assertion \<Rightarrow> ('v, 'a) abs_state assertion"
  (infixl "||" 60) where "(A || B) \<omega> \<longleftrightarrow> A \<omega> \<or> B \<omega>"
+*)
 
 section \<open>Minimal stuff\<close>
 
-definition points_to :: "(('v, 'a) abs_state \<rightharpoonup> 'r) \<Rightarrow> ('v, 'a) abs_state \<Rightarrow> bool" where
-  "points_to r \<omega> \<longleftrightarrow> (\<exists>hl. r \<omega> = Some hl \<and> has_write_perm_only (get_state \<omega>) hl )"
+definition points_to where
+  "points_to r = { \<omega> |\<omega> hl. r \<omega> = Some hl \<and> has_write_perm_only (get_state \<omega>) hl}"
 
 definition points_to_value where
-  "points_to_value r e \<omega> \<longleftrightarrow>(\<exists>hl v. r \<omega> = Some hl \<and> e \<omega> = Some v \<and> has_write_perm_only (get_state \<omega>) hl \<and> has_value (get_state \<omega>) hl v)"
+  "points_to_value r e = { \<omega> |\<omega> hl v. r \<omega> = Some hl \<and> e \<omega> = Some v \<and> has_write_perm_only (get_state \<omega>) hl \<and> has_value (get_state \<omega>) hl v}"
 
+(*
 definition atrue :: "('v, 'a) abs_state assertion" where
   "atrue \<omega> \<longleftrightarrow> True"
-
-definition assertify :: "('v, 'a) abs_state set \<Rightarrow> ('v, 'a) abs_state assertion" where
-  "assertify S \<omega> \<longleftrightarrow> stabilize \<omega> \<in> S"
-
+*)
 
 section \<open>Something else\<close>
 
@@ -276,9 +293,52 @@ abbreviation univ :: "'a \<Rightarrow> ('v, 'a) abs_state set" where
   "univ r \<equiv> UNIV \<times> {r}"
 
 
-
 definition exists_assert :: "('v, 'r) abs_type_context \<Rightarrow> var \<Rightarrow> ('v, 'a) abs_state assertion \<Rightarrow> ('v, 'a) abs_state assertion" where
-  "exists_assert \<Delta> x A \<omega> \<longleftrightarrow> (\<exists>v0 v ty. v0 \<in> ty \<and> get_store \<omega> x = Some v0 \<and> variables \<Delta> x = Some ty \<and> v \<in> ty \<and> A ((Ag ((get_store \<omega>)(x := Some v)), Ag (get_trace \<omega>)), get_state \<omega>))"
+  "exists_assert \<Delta> x A =
+{ \<omega> |\<omega> v0 v ty. v0 \<in> ty \<and> get_store \<omega> x = Some v0 \<and> variables \<Delta> x = Some ty \<and> v \<in> ty \<and> ((Ag ((get_store \<omega>)(x := Some v)), Ag (get_trace \<omega>)), get_state \<omega>) \<in> A}"
+
+
+
+
+
+\<comment> \<open>Hongyi defined these 3 functions for his thesis.
+\<^const>\<open>framed_by_exp\<close> doesn't fully characterize the property "assertion \<^term>\<open>A\<close> frames expression \<^term>\<open>e\<close>",
+in the sense that although \<^term>\<open>e (stabilize_state \<omega>)\<close> has value, it may not equal to \<^term>\<open>e \<omega>\<close>.
+In addition to "frame expression" property, it also excludes evaluation error case. For example,
+expression \<^term>\<open>1 / x\<close> is framed by any assertion, but \<^const>\<open>atrue\<close> does not \<^const>\<open>framed_by_exp\<close>
+it by definition, as there is evaluation error when \<^prop>\<open>x = 0\<close> and it evaluates to \<^const>\<open>None\<close> then.
+Nevertheless, this additional characterization is also essential in defining LocalAssign rule when
+choosing to do substitution in post-condition: this LocalAssign statement must reduce every state
+satisfying pre-condition. As a result, every state satisfying pre-condition must evaluate the expression
+\<^term>\<open>e\<close> not to \<^const>\<open>None\<close>, which is exactly characterized by \<^const>\<open>framed_by_exp\<close>. Moreover,
+substitute_state should be used only when \<^prop>\<open>e \<omega> \<noteq> None\<close>. In SL rules, this is guaranteed by \<^const>\<open>framed_by_exp\<close>.
+\<close>
+
+definition assertion_frame_exp :: "('v, 'a) abs_state assertion \<Rightarrow> (('v, 'a) abs_state, 'v) exp \<Rightarrow> bool" where
+  "assertion_frame_exp A e \<longleftrightarrow> (\<forall>\<omega> \<in> A. e \<omega> = e (stabilize \<omega>))"
+
+definition substitute_var_state :: "var \<Rightarrow> (('v, 'a) abs_state, 'v) exp \<Rightarrow> ('v, 'a) abs_state \<Rightarrow> ('v, 'a) abs_state" where
+  "substitute_var_state x e \<omega> = ((Ag ((get_store \<omega>)(x := e \<omega>)), Ag (get_trace \<omega>)), get_state \<omega>)"
+
+definition post_substitute_var_assert :: "var \<Rightarrow> (('v, 'a) abs_state, 'v) exp \<Rightarrow> ('v, 'a) abs_state assertion \<Rightarrow> ('v, 'a) abs_state assertion" where
+  "post_substitute_var_assert x e A = { \<omega>' |\<omega> \<omega>'. \<omega> \<in> A \<and> \<omega>' = substitute_var_state x e \<omega>}"
+
+definition set_value_state :: "'r \<Rightarrow> 'v \<Rightarrow> ('v, 'a) abs_state \<Rightarrow> ('v, 'a) abs_state" where
+  "set_value_state l v \<omega> = ((Ag (get_store \<omega>), Ag (get_trace \<omega>)), set_value (get_state \<omega>) l v)"
+
+definition substitute_field_state :: "(('v, 'a) abs_state \<rightharpoonup> 'r) \<Rightarrow> (('v, 'a) abs_state, 'v) exp \<Rightarrow> ('v, 'a) abs_state \<Rightarrow> ('v, 'a) abs_state" where
+  "substitute_field_state r e \<omega> = set_value_state (the (r \<omega>)) (the (e \<omega>)) \<omega>"
+
+definition post_substitute_field_assert :: "(('v, 'a) abs_state \<rightharpoonup> 'r) \<Rightarrow> (('v, 'a) abs_state, 'v) exp \<Rightarrow> ('v, 'a) abs_state assertion \<Rightarrow> ('v, 'a) abs_state assertion" where
+  "post_substitute_field_assert r e A = { \<omega>' |\<omega>' \<omega>. \<omega> \<in> A \<and> \<omega>' = substitute_field_state r e \<omega>}"
+
+
+
+
+
+
+
+
 
 section \<open>SL Proof\<close>
 
@@ -292,32 +352,41 @@ inductive SL_proof :: "('v, 'r) abs_type_context \<Rightarrow> ('v, 'a) abs_stat
   RuleSkip: "self_framing A \<Longrightarrow> _ \<turnstile> [A] Skip [A]"
 \<comment>\<open>Because no frame rule, needs A on both sides.\<close>
 
-| RuleInhale: "self_framing A \<Longrightarrow> framed_by A P \<Longrightarrow> _ \<turnstile> [A] Inhale P [A && P]"
+| RuleInhale: "self_framing A \<Longrightarrow> framed_by A P \<Longrightarrow> _ \<turnstile> [A] Inhale P [A \<otimes> P]"
 \<comment>\<open>P framed by A ensures that A && P is self-framing.\<close>
 
-| RuleExhale: "self_framing B \<Longrightarrow> entails B (A && P) \<Longrightarrow> self_framing A \<Longrightarrow> _ \<turnstile> [B] Exhale P [A]"
+| RuleExhale: "self_framing B \<Longrightarrow> entails B (A \<otimes> P) \<Longrightarrow> self_framing A \<Longrightarrow> _ \<turnstile> [B] Exhale P [A]"
 \<comment>\<open>Exhale can lose information, because we're forced to factorize the set, which is why the entails is needed.
 Example:
 {a1 + p1, a2 + p2} \<longlonglongrightarrow> {a1, a2}
 <A * P> = {a1 + p1, a2 + p2, a1 + p2, a2 + p1} \<longlonglongrightarrow> {a1, a2}\<close>
+
 
 | RuleAssert: "self_framing A \<Longrightarrow> entails A P \<Longrightarrow> _ \<turnstile> [A] Assert P [A]"
 \<comment>\<open>Assert does not behave like exhale: It forces the *whole* heap to satisfy P.
 Because there is not frame rule, it can be used to express leak checks, or absence of obligations.\<close>
 
 | RuleHavoc: "self_framing A \<Longrightarrow> \<Delta> \<turnstile> [A] Havoc x [exists_assert \<Delta> x A]"
+
 (*
 | RuleHavoc: "self_framing A \<Longrightarrow> self_framing B \<Longrightarrow> entails A B \<Longrightarrow> free_vars \<Delta> B \<subseteq> free_vars \<Delta> A - {x} \<Longrightarrow> \<Delta> \<turnstile> [A] Havoc x [B]"
 *)
 \<comment>\<open>Entails needed, because we lose information. The strongest post might be \<exists>x. A, but does not seem more useful.\<close>
 
+\<comment> \<open>
 | RuleFieldAssignHeapIndep:
   "\<lbrakk> self_framing A; framed_by_exp A r; framed_by_exp A e; depends_on_ag_store_only r; depends_on_ag_store_only e \<rbrakk>
   \<Longrightarrow> \<Delta> \<turnstile> [A && points_to r] FieldAssign r e [A && points_to_value r e]"
+Replaced by the new uniform one below in Hongyi's thesis.\<close>
 
+| RuleFieldAssign: "\<lbrakk> self_framing (A \<otimes> points_to r); framed_by_exp (A \<otimes> points_to r) e; assertion_frame_exp (A \<otimes> points_to r) e \<rbrakk>
+  \<Longrightarrow> _ \<turnstile> [A \<otimes> points_to r] FieldAssign r e [post_substitute_field_assert r e (A \<otimes> points_to r)]"
 
+\<comment> \<open>Replaced to the new one above in Hongyi's thesis. The new one simply simulates reduction of this statement, with assumptions ensuring the simulation doesn't cause error.
 | RuleFieldAssign: "\<lbrakk> self_framing (A && points_to_value r e') ; framed_by_exp (A && points_to r) e \<rbrakk>
-  \<Longrightarrow> \<Delta> \<turnstile> [A && points_to_value r e'] FieldAssign r e [A && points_to_value r e]"
+  \<Longrightarrow> \<Delta> \<turnstile> [A && points_to_value r e'] FieldAssign r e [A && points_to_value r e]"\<close>
+
+
 \<comment>\<open>Like inhale and the if rule, needs to frame r and e.
 Interestingly, does not work if we only have
 - self_framing A
@@ -343,9 +412,6 @@ x.f := ...
 --> "issue" if location of "e" depends on the value of e
 
 
-
-
-
 x.f.f := ...
 --> "issue" if location of "x.f.f" depends on the value of x.f.f
 --> In Viper, location of "x.f.f" depends on the value of x.f
@@ -362,17 +428,13 @@ x = 0 && (\<exists>v. x.f \<mapsto> v /\ v
 acc(x.f) && x.f = x
 [x.f.f := ...]
 
-
-
-Might need an entailment...
-
-Otherwise:
-\<close>
+Might need an entailment...\<close>
 
 | RuleSeq: "\<lbrakk> \<Delta> \<turnstile> [A] C1 [R] ; \<Delta> \<turnstile> [R] C2 [B] \<rbrakk> \<Longrightarrow> \<Delta> \<turnstile> [A] Seq C1 C2 [B]"
-| RuleIf: "\<lbrakk> framed_by_exp A b; \<Delta> \<turnstile> [A \<and>\<and> (pure_assertify b)] C1 [B1] ; \<Delta> \<turnstile> [A \<and>\<and> (pure_assertify (negate b))] C2 [B2] \<rbrakk>
+(*
+| RuleIf: "\<lbrakk> framed_by_exp A b; \<Delta> \<turnstile> [A \<and>\<and> (pure_Stabilize b)] C1 [B1] ; \<Delta> \<turnstile> [A \<and>\<and> (pure_Stabilize (negate b))] C2 [B2] \<rbrakk>
   \<Longrightarrow> \<Delta> \<turnstile> [A] If b C1 C2 [B1 || B2]"
-
+*)
 
 
 (*
